00Utils/Unification/UnifiableTerm.thy
@@ -1,0 +1,88 @@
+theory UnifiableTerm
+  imports "../Utils" "../Variable"
+begin
+
+section \<open>Unification\<close>
+
+text \<open>Before we can do typechecking, we need a key tool: the unification algorithm. Our treatment 
+here is based on Pierce [5].\<close>
+
+subsection \<open>Unifiable terms\<close>
+
+text \<open>The unification algorithm acts on terms, which for clarity we will always refer to as such (in
+contrast to our compilation languages' "expressions". In theory, we do not need the full generality 
+of the treatment here, since we only ever unify terms representing our limited selection of types. 
+However, specializing the term language would only simplify the (quite straightforward) conversion 
+between types and terms, while complicating the unification algorithm itself, which is where the 
+subtlety already lies anyway. (It would also prevent us from reusing the algorithm if we wished to 
+add unification elsewhere - adding a logic-programming component to the source language, perhaps.) 
+We therefore define unifiable terms in a very general way:\<close>
+
+datatype uterm = 
+  Var var
+  | Ctor string "uterm list"
+
+fun uvars :: "uterm \<Rightarrow> var set" 
+and uvarss :: "uterm list \<Rightarrow> var set" where
+  "uvars (Var x) = {x}"
+| "uvars (Ctor k \<tau>s) = uvarss \<tau>s"
+| "uvarss [] = {}"
+| "uvarss (\<tau> # \<tau>s) = uvars \<tau> \<union> uvarss \<tau>s"
+
+lemma finite_uvars [simp]: "finite (uvars \<tau>)"
+  and "finite (uvarss \<tau>s)"
+  by (induction \<tau> and \<tau>s rule: uvars_uvarss.induct) simp_all
+
+text \<open>"Structural" properties are those that relate purely to the constructor well-formedness of 
+terms; that is, the names of constructors and the number of arguments to them, but not which 
+constructors or variables exist inside of which. We will use this to show that the well-formedness 
+of terms representing types is preserved through substitution.\<close>
+
+definition structural :: "(uterm \<Rightarrow> bool) \<Rightarrow> bool" where
+  "structural P = (\<exists>f. \<forall>k es. P (Ctor k es) = (list_all P es \<and> f k (length es)))"
+
+text \<open>We also define constraints, pairs of terms which must be unified with each other. Functions on 
+terms extend to constraints in an obvious way.\<close>
+
+type_synonym constraint = "(uterm \<times> uterm) list"
+
+fun constr_vars :: "constraint \<Rightarrow> var set" where
+  "constr_vars [] = {}"
+| "constr_vars ((\<tau>\<^sub>1, \<tau>\<^sub>2) # \<kappa>) = uvars \<tau>\<^sub>1 \<union> uvars \<tau>\<^sub>2 \<union> constr_vars \<kappa>"
+
+lemma finite_constr_vars [simp]: "finite (constr_vars \<kappa>)"
+  by (induction \<kappa> rule: constr_vars.induct) simp_all
+
+lemma constr_vars_append [simp]: "constr_vars (\<kappa>\<^sub>1 @ \<kappa>\<^sub>2) = constr_vars \<kappa>\<^sub>1 \<union> constr_vars \<kappa>\<^sub>2"
+  by (induction \<kappa>\<^sub>1 rule: constr_vars.induct) auto
+
+lemma constr_vars_zip [simp]: "length \<tau>s\<^sub>1 = length \<tau>s\<^sub>2 \<Longrightarrow> 
+  constr_vars (zip \<tau>s\<^sub>1 \<tau>s\<^sub>2) = uvarss \<tau>s\<^sub>1 \<union> uvarss \<tau>s\<^sub>2"
+proof (induction \<tau>s\<^sub>1 arbitrary: \<tau>s\<^sub>2)
+  case (Cons \<tau>\<^sub>1 \<tau>s\<^sub>1)
+  thus ?case by (induction \<tau>s\<^sub>2) auto
+qed simp_all
+
+text \<open>\<open>list_ctor_count\<close> is used in one very specific place for the termination of the unification 
+algorithm, hence its slightly odd definition ignoring the right-hand sides of constraint equations.\<close>
+
+primrec ctor_count :: "uterm \<Rightarrow> nat" where
+  "ctor_count (Var x) = 0"
+| "ctor_count (Ctor k \<tau>s) = Suc (sum_list (map ctor_count \<tau>s))"
+
+fun constr_ctor_count :: "constraint \<Rightarrow> nat" where
+  "constr_ctor_count [] = 0"
+| "constr_ctor_count ((\<tau>\<^sub>1, \<tau>\<^sub>2) # \<kappa>) = ctor_count \<tau>\<^sub>1 + constr_ctor_count \<kappa>"
+
+lemma constr_ctor_count_append [simp]: "constr_ctor_count (ess\<^sub>1 @ ess\<^sub>2) = 
+    constr_ctor_count ess\<^sub>1 + constr_ctor_count ess\<^sub>2"
+  by (induction ess\<^sub>1 rule: constr_ctor_count.induct) simp_all
+
+lemma constr_ctor_count_zip [simp]: "length \<tau>s\<^sub>1 = length \<tau>s\<^sub>2 \<Longrightarrow> 
+  constr_ctor_count (zip \<tau>s\<^sub>1 \<tau>s\<^sub>2) = sum_list (map ctor_count \<tau>s\<^sub>1)"
+proof (induction \<tau>s\<^sub>1 arbitrary: \<tau>s\<^sub>2)
+  case (Cons \<tau>\<^sub>1 \<tau>s\<^sub>1)
+  thus ?case by (induction \<tau>s\<^sub>2) simp_all
+qed simp_all
+
+end
